Flapjack/Test/PipelineDiagnostics.lean
@@ -1,0 +1,32 @@
+import Flapjack.RiscV.PipelineDiagnostics
+
+namespace Flapjack
+
+open RiscV
+
+def pipelineDiagnosticsConfig : WordStackConfig :=
+  { locations := [(0, .register 5), (1, .register 6),
+      (2, .register 7), (3, .register 8)]
+    scratch := 31
+    stackBase := 10 }
+
+example :
+    RiscV.pipelineWordFunctionsToStackChecked (width := 64)
+      [(17, [], (.alloc 0 ([], []) : WordProg (RiscV.Word 64)))] =
+        .error { sectionId := 17, path := [], feature := .alloc } := by
+  simp [RiscV.pipelineWordFunctionsToStackChecked,
+    RiscV.wordStackIdentityConfig, RiscV.wordToStackProgWordChecked,
+    RiscV.wordToStackProgNatChecked, RiscV.wordToStackProgNat,
+    RiscV.wordProgFirstUnsupported, RiscV.wordProgToNat]
+
+example :
+    RiscV.pipelineWordFunctionsToStackChecked (width := 64)
+      [(23, [], ((.seq .skip (.storeConsts 0 1 2 3 [])) :
+        WordProg (RiscV.Word 64)))] =
+        .error { sectionId := 23, path := [1], feature := .storeConsts } := by
+  simp [RiscV.pipelineWordFunctionsToStackChecked,
+    RiscV.wordStackIdentityConfig, RiscV.wordToStackProgWordChecked,
+    RiscV.wordToStackProgNatChecked, RiscV.wordToStackProgNat,
+    RiscV.wordProgFirstUnsupported, RiscV.wordProgToNat]
+
+end Flapjack
